Some progress on tailcallproof
I tried to change the extension into an injection because currently an extension
can only have a 'flat´ stack injection, which is not the case for Tailcall. The
problem is that I can't assume the injection is the flat injection because
that's not preserved by external call steps. (Actually it should but it's not
proven anywhere).

A possible step would be to generalize the memory injection function into an
arbitrary j but I would still need to know that the globals are in flat inj and
that the stack blocks inject into their target counterpart.

If that's too complicated, generalize the extensions in the memory model so that
they can be parameterized by a stack injection function, not necessarily the
flat stack injection.

backend/Tailcallproof.v
@@ -218,6 +218,33 @@ Existing Instance inject_perm_all.
 Variable prog tprog: program.
 Hypothesis TRANSL: match_prog prog tprog.
 
+Definition regs_inject (j: meminj) (rs1 rs2: Regmap.t val) :=
+  forall r,
+    Val.inject j (rs1 # r) (rs2 # r).
+
+Lemma meminj_preserves_globals_flat {F V} (g: Genv.t F V) m:
+  Ple (Genv.genv_next g) (Mem.nextblock m) ->
+  meminj_preserves_globals g (Mem.flat_inj (Mem.nextblock m)).
+Proof.
+  intros PLE.
+  split; [|split].
+  - intros id b FS.
+    unfold Genv.find_symbol in FS.
+    eapply Genv.genv_symb_range in FS.
+    unfold Mem.flat_inj; rewrite pred_dec_true; auto. xomega.
+  - intros id b FVI.
+    unfold Genv.find_var_info in FVI.
+    repeat destr_in FVI.
+    eapply Genv.genv_defs_range in Heqo.
+    unfold Mem.flat_inj; rewrite pred_dec_true; auto. xomega.
+  - intros b1 b2 delta gv FVI FI.
+    unfold Genv.find_var_info in FVI.
+    repeat destr_in FVI.
+    eapply Genv.genv_defs_range in Heqo.
+    unfold Mem.flat_inj in FI; destr_in FI. 
+Qed.
+
+
 Let ge := Genv.globalenv prog.
 Let tge := Genv.globalenv tprog.
 
@@ -262,16 +289,17 @@ Proof.
 Qed.
 
 Lemma find_function_translated:
-  forall ros rs rs' f,
+  forall ros rs rs' f m,
   find_function ge ros rs = Some f ->
-  regs_lessdef rs rs' ->
+  regs_inject (Mem.flat_inj (Mem.nextblock m)) rs rs' ->
   find_function tge ros rs' = Some (transf_fundef f).
 Proof.
-  intros until f; destruct ros; simpl.
+  intros until m; destruct ros; simpl.
   intros.
   assert (rs'#r = rs#r).
     exploit Genv.find_funct_inv; eauto. intros [b EQ].
-    generalize (H0 r). rewrite EQ. intro LD. inv LD. auto.
+    generalize (H0 r). rewrite EQ. intro LD. inv LD.
+    unfold Mem.flat_inj in H4. repeat destr_in H4. reflexivity.
   rewrite H1. apply functions_translated; auto.
   rewrite symbols_preserved. destruct (Genv.find_symbol ge i); intros.
   apply funct_ptr_translated; auto.
@@ -312,22 +340,55 @@ We first define the simulation invariant between call stacks.
 The first two cases are standard, but the third case corresponds
 to a frame that was eliminated by the transformation. *)
 
-Inductive match_stackframes: list stackframe -> list stackframe -> Prop :=
-  | match_stackframes_nil:
-      match_stackframes nil nil
-  | match_stackframes_normal: forall stk stk' res sp pc rs rs' f,
-      match_stackframes stk stk' ->
-      regs_lessdef rs rs' ->
-      match_stackframes
+
+(* The list of boolean records whether the source frame has a corresponding
+counterpart in the target stack ([true]) or not ([false]). This will later be used
+to specify the shape of the stack injection function [g]. *)
+Inductive match_stackframes: meminj -> list bool -> list stackframe -> list stackframe -> Prop :=
+  | match_stackframes_nil j:
+      match_stackframes j nil nil nil
+  | match_stackframes_normal: forall j l stk stk' res sp pc rs rs' f,
+      match_stackframes j l stk stk' ->
+      regs_inject j rs rs' ->
+      j sp = Some (sp,0) ->
+      match_stackframes j (true::l)
         (Stackframe res f (Vptr sp Ptrofs.zero) pc rs :: stk)
         (Stackframe res (transf_function f) (Vptr sp Ptrofs.zero) pc rs' :: stk')
-  | match_stackframes_tail: forall stk stk' res sp pc rs f,
-      match_stackframes stk stk' ->
+  | match_stackframes_tail: forall j l stk stk' res sp pc rs f,
+      match_stackframes j l stk stk' ->
       is_return_spec f pc res ->
       f.(fn_stacksize) = 0 ->
-      match_stackframes
+      match_stackframes j (false::l)
         (Stackframe res f (Vptr sp Ptrofs.zero) pc rs :: stk)
         stk'.
+
+(* Specifying the shape of stack injection functions *)
+
+Fixpoint compat_frameinj_rec (l: list bool) (g: frameinj) (ns nt: nat) :=
+  match l with
+    nil => forall i j (LE: (ns <= i)%nat) (Gi: g i = Some j), (nt <= j)%nat
+  | true::l =>
+    g ns = Some nt /\ compat_frameinj_rec l g (S ns) (S nt)
+  | false::l =>
+    g ns = None /\ compat_frameinj_rec l g (S ns) nt
+  end.
+
+Definition compat_frameinj l g := compat_frameinj_rec l g O O.
+
+Lemma compat_frameinj_rec_above:
+  forall l g ns nt (CFG: compat_frameinj_rec l g ns nt)
+    i j (Gi: g i = Some j) (LE: (ns <= i)%nat),
+    (nt <= j)%nat.
+Proof.
+  induction l; simpl; intros; eauto.
+  destruct a; destruct CFG as (GNS & GABOVE).
+  - destruct (Nat.eq_dec ns i); subst; auto.
+    + rewrite GNS in Gi; inv Gi; auto.
+    + eapply IHl in GABOVE. 2: apply Gi. 2: omega. omega.
+  - destruct (Nat.eq_dec ns i); subst; auto. 
+    + congruence.
+    + eapply IHl in GABOVE. 2: apply Gi. 2: omega. omega.
+Qed.
 
 (** Here is the invariant relating two states.  The first three
   cases are standard.  Note the ``less defined than'' conditions
@@ -336,35 +397,95 @@ Inductive match_stackframes: list stackframe -> list stackframe -> Prop :=
 
 Inductive match_states: state -> state -> Prop :=
   | match_states_normal:
-      forall s sp pc rs m s' rs' m' f
-             (STACKS: match_stackframes s s')
-             (RLD: regs_lessdef rs rs')
-             (MLD: Mem.extends m m'),
+      forall s sp pc rs m s' rs' m' f g l
+             (STACKS: match_stackframes (Mem.flat_inj (Mem.nextblock m)) l s s')
+             (RLD: regs_inject (Mem.flat_inj (Mem.nextblock m)) rs rs')
+             (MLD: Mem.inject (Mem.flat_inj (Mem.nextblock m)) g m m')
+             (CFG: compat_frameinj (true::l) g),
       match_states (State s f (Vptr sp Ptrofs.zero) pc rs m)
                    (State s' (transf_function f) (Vptr sp Ptrofs.zero) pc rs' m')
   | match_states_call:
-      forall s f args m s' args' m' sz,
-      match_stackframes s s' ->
-      Val.lessdef_list args args' ->
-      Mem.extends m m' ->
+      forall s f args m s' args' m' sz g l
+        (MS: match_stackframes (Mem.flat_inj (Mem.nextblock m)) l s s')
+        (LDargs: Val.inject_list (Mem.flat_inj (Mem.nextblock m)) args args')
+        (MLD: Mem.inject (Mem.flat_inj (Mem.nextblock m)) g m m')
+        (CFG: compat_frameinj l g),
       match_states (Callstate s f args m sz)
                    (Callstate s' (transf_fundef f) args' m' sz)
   | match_states_return:
-      forall s v m s' v' m',
-      match_stackframes s s' ->
-      Val.lessdef v v' ->
-      Mem.extends m m' ->
-      match_states (Returnstate s v m)
-                   (Returnstate s' v' m')
+      forall s v m s' v' m' g l
+        (MS: match_stackframes (Mem.flat_inj (Mem.nextblock m)) l s s')
+        (LDret: Val.inject (Mem.flat_inj (Mem.nextblock m)) v v')
+        (MLD: Mem.inject (Mem.flat_inj (Mem.nextblock m)) g m m')
+        (CFG: compat_frameinj (true::l) g),
+        match_states (Returnstate s v m)
+                     (Returnstate s' v' m')
   | match_states_interm:
-      forall s sp pc rs m s' m' f r v'
-             (STACKS: match_stackframes s s')
-             (MLD: Mem.extends m m'),
-      is_return_spec f pc r ->
-      f.(fn_stacksize) = 0 ->
-      Val.lessdef (rs#r) v' ->
-      match_states (State s f (Vptr sp Ptrofs.zero) pc rs m)
-                   (Returnstate s' v' m').
+      forall s sp pc rs m s' m' f r v' g l
+             (STACKS: match_stackframes (Mem.flat_inj (Mem.nextblock m)) l s s')
+             (MLD: Mem.inject (Mem.flat_inj (Mem.nextblock m)) g m m')
+             (RETspec: is_return_spec f pc r)
+             (SZzero: f.(fn_stacksize) = 0)
+             (LDret: Val.inject (Mem.flat_inj (Mem.nextblock m)) (rs#r) v')
+             (CFG: compat_frameinj l g),
+        match_states (State s f (Vptr sp Ptrofs.zero) pc rs m)
+                     (Returnstate s' v' m').
+
+Definition mem_state (s: state) : mem :=
+  match s with
+    State _ _ _ _ _ m
+  | Callstate _ _ _ m _
+  | Returnstate _ _ m => m
+  end.
+
+Definition match_state_ge {F V} (g: Genv.t F V) (s: state) :=
+  Ple (Genv.genv_next g) (Mem.nextblock (mem_state s)).
+
+Definition current_sp_state (s: state) : option (block * Z) :=
+  match s with
+    State _ f (Vptr sp _) _ _ _ => Some (sp, fn_stacksize f)
+  | _ => None
+  end.
+
+Definition stackblocks_of_stackframe (sf: stackframe) : option (block * Z) :=
+  match sf with
+  | (Stackframe _ f (Vptr sp _) _ _) => Some (sp,fn_stacksize f)
+  | _ => None
+  end.
+
+
+Definition stackframes_state (s: state) : list stackframe :=
+  match s with
+    State stk _ _ _ _ _
+  | Callstate stk _ _ _ _
+  | Returnstate stk _ _ => stk
+  end.
+
+
+Definition stack_blocks_of_state (s: state) : list (option (block * Z)) :=
+  current_sp_state s :: map stackblocks_of_stackframe (stackframes_state s).
+
+Definition sp_valid (s : state) : Prop :=
+  Forall (fun bz => match bz with
+                   Some (b,z) => Mem.valid_block (mem_state s) b
+                 | None => False
+                 end) (stack_blocks_of_state s).
+
+Definition match_stack_adt (s: state) :=
+  let stk := Mem.stack_adt (mem_state s) in
+  let sbl := stack_blocks_of_state s in
+  exists sprog sinit,
+    stk = sprog ++ sinit /\
+    list_forall2 (fun (f: frame_adt) obz =>
+                    match obz with
+                      Some (b,z) =>
+                      map fst (frame_adt_blocks f) = b :: nil /\
+                      forall o k p,
+                        Mem.perm (mem_state s) b o k p ->
+                        0 <= o < z
+                    | None => False
+                    end
+                 ) sprog sbl.
 
 (** The last case of [match_states] corresponds to the execution
   of a move/nop/return sequence in the original code that was
@@ -405,11 +526,57 @@ Ltac EliminatedInstr :=
 (** The proof of semantic preservation, then, is a simulation diagram
   of the ``option'' kind. *)
 
+
+Lemma regs_inject_regs:
+  forall j rs1 rs2, regs_inject j rs1 rs2 ->
+  forall rl, Val.inject_list j rs1##rl rs2##rl.
+Proof.
+  induction rl; constructor; auto.
+Qed.
+
+Lemma set_reg_inject:
+  forall j r v1 v2 rs1 rs2,
+  Val.inject j v1 v2 -> regs_inject j rs1 rs2 -> regs_inject j (rs1#r <- v1) (rs2#r <- v2).
+Proof.
+  intros; red; intros. repeat rewrite Regmap.gsspec.
+  destruct (peq r0 r); auto.
+Qed.
+
+Lemma set_res_inject:
+  forall j res v1 v2 rs1 rs2,
+  Val.inject j v1 v2 -> regs_inject j rs1 rs2 ->
+  regs_inject j (regmap_setres res v1 rs1) (regmap_setres res v2 rs2).
+Proof.
+  intros. destruct res; simpl; auto. apply set_reg_inject; auto.
+Qed.
+
+
+
+
+
 Variable fn_stack_requirements: ident -> Z.
+
+
+Lemma ros_is_function_transf:
+  forall j ros rs rs' id,
+    meminj_preserves_globals ge j ->
+    ros_is_function ge ros rs id ->
+    regs_inject j rs rs' ->
+    ros_is_function tge ros rs' id.
+Proof.
+  unfold ros_is_function. intros.
+  destr_in H0. simpl.
+  destruct H0 as (b & o & RS & FS).
+  specialize (H1 r). rewrite RS in H1; inv H1.
+  eexists; eexists; split; eauto.
+  rewrite symbols_preserved. rewrite FS.
+  f_equal.
+  destruct H. apply H in FS. rewrite FS in H4; inv H4. auto.
+Qed.
 
 Lemma transf_step_correct:
   forall s1 t s2, step fn_stack_requirements ge s1 t s2 ->
-  forall s1' (MS: match_states s1 s1'),
+  forall s1' (MS: match_states s1 s1') (MSG: match_state_ge ge s1) (SPV: sp_valid s1) (MSA: match_stack_adt s1) (MSA': match_stack_adt s1'),
   (exists s2', step fn_stack_requirements tge s1' t s2' /\ match_states s2 s2')
   \/ (measure s2 < measure s1 /\ t = E0 /\ match_states s2 s1')%nat.
 Proof.
@@ -417,7 +584,7 @@ Proof.
 
 - (* nop *)
   TransfInstr. left. econstructor; split.
-  eapply exec_Inop; eauto. constructor; auto.
+  eapply exec_Inop; eauto. econstructor; eauto.
 - (* eliminated nop *)
   assert (s0 = pc') by congruence. subst s0.
   right. split. simpl. omega. split. auto.
@@ -425,13 +592,17 @@ Proof.
 
 - (* op *)
   TransfInstr.
-  assert (Val.lessdef_list (rs##args) (rs'##args)). apply regs_lessdef_regs; auto.
-  exploit eval_operation_lessdef; eauto.
+  assert (Val.inject_list (Mem.flat_inj (Mem.nextblock m)) (rs##args) (rs'##args)). apply regs_inject_regs; auto.
+  exploit eval_operation_inject; eauto.
+  eapply meminj_preserves_globals_flat; eauto.
+  unfold Mem.flat_inj. rewrite pred_dec_true. reflexivity.
+  inv SPV. eauto.
   intros [v' [EVAL' VLD]].
   left. exists (State s' (transf_function f) (Vptr sp0 Ptrofs.zero) pc' (rs'#res <- v') m'); split.
   eapply exec_Iop; eauto.  rewrite <- EVAL'.
+  rewrite eval_shift_stack_operation.
   apply eval_operation_preserved. exact symbols_preserved.
-  econstructor; eauto. apply set_reg_lessdef; auto.
+  econstructor; eauto. apply set_reg_inject; auto.
 - (* eliminated move *)
   rewrite H1 in H. clear H1. inv H.
   right. split. simpl. omega. split. auto.
@@ -439,74 +610,232 @@ Proof.
 
 - (* load *)
   TransfInstr.
-  assert (Val.lessdef_list (rs##args) (rs'##args)). apply regs_lessdef_regs; auto.
-  exploit eval_addressing_lessdef; eauto.
+  assert (Val.inject_list (Mem.flat_inj (Mem.nextblock m)) (rs##args) (rs'##args)). apply regs_inject_regs; auto.
+  exploit eval_addressing_inject; eauto.
+  eapply meminj_preserves_globals_flat; eauto.
+  unfold Mem.flat_inj; rewrite pred_dec_true; auto.   inv SPV. eauto.
   intros [a' [ADDR' ALD]].
-  exploit Mem.loadv_extends; eauto.
+  exploit Mem.loadv_inject; eauto.
   intros [v' [LOAD' VLD]].
   left. exists (State s' (transf_function f) (Vptr sp0 Ptrofs.zero) pc' (rs'#dst <- v') m'); split.
   eapply exec_Iload with (a0 := a'). eauto.  rewrite <- ADDR'.
+  rewrite eval_shift_stack_addressing.
   apply eval_addressing_preserved. exact symbols_preserved. eauto.
-  econstructor; eauto. apply set_reg_lessdef; auto.
+  econstructor; eauto. apply set_reg_inject; auto.
 
 - (* store *)
   TransfInstr.
-  assert (Val.lessdef_list (rs##args) (rs'##args)). apply regs_lessdef_regs; auto.
-  exploit eval_addressing_lessdef; eauto.
+  assert (Val.inject_list (Mem.flat_inj (Mem.nextblock m)) (rs##args) (rs'##args)). apply regs_inject_regs; auto.
+  exploit eval_addressing_inject; eauto.
+  eapply meminj_preserves_globals_flat; eauto.
+  unfold Mem.flat_inj; rewrite pred_dec_true; auto. inv SPV. eauto.
   intros [a' [ADDR' ALD]].
-  exploit Mem.storev_extends. 2: eexact H1. eauto. eauto. apply RLD.
+  exploit Mem.storev_mapped_inject. 2: eexact H1. eauto. eauto. apply RLD.
   intros [m'1 [STORE' MLD']].
   left. exists (State s' (transf_function f) (Vptr sp0 Ptrofs.zero) pc' rs' m'1); split.
   eapply exec_Istore with (a0 := a'). eauto.  rewrite <- ADDR'.
+  rewrite eval_shift_stack_addressing.
   apply eval_addressing_preserved. exact symbols_preserved. eauto.
   destruct a; simpl in H1; try discriminate.
   econstructor; eauto.
+  erewrite Mem.nextblock_store; eauto.
+  erewrite Mem.nextblock_store; eauto.
+  erewrite Mem.nextblock_store; eauto.
 
 - (* call *)
   exploit find_function_translated; eauto. intro FIND'.
   TransfInstr.
 + (* call turned tailcall *)
-  assert ({ m'' | Mem.free m' sp0 0 (fn_stacksize (transf_function f)) = Some m''}).
+  assert (X: { m'' | Mem.free m' sp0 0 (fn_stacksize (transf_function f)) = Some m''}).
+  {
     apply Mem.range_perm_free. rewrite stacksize_preserved. rewrite H7.
     red; intros; omegaContradiction.
+  } 
   destruct X as [m'' FREE].
-  left. exists (Callstate s' (transf_fundef fd) (rs'##args) m''); split.
-  eapply exec_Itailcall; eauto. apply sig_preserved.
-  constructor. eapply match_stackframes_tail; eauto. apply regs_lessdef_regs; auto.
-  eapply Mem.free_right_extends; eauto.
-  rewrite stacksize_preserved. rewrite H7. intros. omegaContradiction.
+  generalize (Mem.free_right_inject _ _ _ _ _ _ _ _ MLD FREE). intro FINJ.
+  trim FINJ.
+  {
+    unfold Mem.flat_inj.
+    intros b1 delta ofs k p FI PERM RNG.
+    repeat destr_in FI.
+    rewrite stacksize_preserved in RNG. rewrite H7 in RNG. omega.
+  }
+  destruct MSA as (sprog & sinit & EQstk & LF2).
+  inv LF2. simpl in EQstk.
+  destruct MSA' as (sprog' & sinit' & EQstk' & LF2').
+  inv LF2'. simpl in EQstk'.
+  edestruct (Mem.unrecord_stack_block_succeeds m'') as (m2' & USB & EQ).
+  erewrite Mem.free_stack_blocks; eauto.
+  generalize (Mem.unrecord_stack_block_inject_right _ _ _ _ m2' FINJ). intro UINJ.
+  trim UINJ.
+  {
+    rewrite EQstk. unfold is_stack_top. simpl.
+    destruct H4 as (frame_blocks & perm_stack).
+    rewrite frame_blocks. intros b [A|[]]; inv A.
+    intros (o & k & p & PERM).
+    apply perm_stack in PERM. rewrite H7 in PERM. omega.
+  }
+  trim UINJ.
+  {
+    red in CFG. simpl in CFG.
+    intros i j Gi LT.
+    eapply compat_frameinj_rec_above in Gi. 2: apply CFG. omega. omega.
+  }
+  trim UINJ. apply CFG.
+  trim UINJ. eauto.
+  left. exists (Callstate s' (transf_fundef fd) (rs'##args) m2' (fn_stack_requirements id)); split.
+  eapply exec_Itailcall; eauto.
+  {
+    eapply ros_is_function_transf; eauto.
+    eapply meminj_preserves_globals_flat; eauto.
+  }
+  apply sig_preserved.
+  econstructor. eapply match_stackframes_tail; eauto. apply regs_inject_regs; auto.
+  eauto.
+  {
+    revert CFG.
+
+    Lemma compat_frameinj_pop_right_rec:
+      forall g l ns nt
+        (CFR: compat_frameinj_rec l g ns (S nt))
+        g' (G'spec: forall i, (ns <= i)%nat -> g' i = option_map pred (g i)),
+        compat_frameinj_rec l g' ns nt.
+    Proof.
+      induction l; simpl; intros; eauto.
+      - rewrite G'spec in Gi; auto.
+        unfold option_map in Gi; repeat destr_in Gi.
+        eapply CFR in Heqo. omega. auto.
+      - destr; destruct CFR as (Gn & CFR).
+        + split.
+          * rewrite G'spec; auto.
+            unfold option_map. rewrite Gn. reflexivity.
+          * eapply IHl; eauto.
+            intros; apply G'spec. omega.
+        + split.
+          * rewrite G'spec; auto.
+            unfold option_map. rewrite Gn. reflexivity.
+          * eapply IHl; eauto.
+            intros; apply G'spec. omega.
+    Qed.
+
+    Lemma compat_frameinj_pop_right:
+      forall g l,
+        compat_frameinj (true :: l) g ->
+        compat_frameinj (false :: l) (fun n : nat => if Nat.eq_dec n 0 then None else option_map Init.Nat.pred (g n)).
+    Proof.
+      intros g l (A & B); split; simpl; auto.
+      eapply compat_frameinj_pop_right_rec; eauto.
+      intros. destr. omega.
+    Qed.
+    eapply compat_frameinj_pop_right; eauto.
+
+  }
+
 + (* call that remains a call *)
   left. exists (Callstate (Stackframe res (transf_function f) (Vptr sp0 Ptrofs.zero) pc' rs' :: s')
-                          (transf_fundef fd) (rs'##args) m'); split.
-  eapply exec_Icall; eauto. apply sig_preserved.
-  constructor. constructor; auto. apply regs_lessdef_regs; auto. auto.
+                          (transf_fundef fd) (rs'##args) m' (fn_stack_requirements id)); split.
+  eapply exec_Icall; eauto.
+  eapply ros_is_function_transf; eauto.
+  eapply meminj_preserves_globals_flat; eauto.
+  apply sig_preserved.
+  econstructor. constructor; eauto.
+  unfold Mem.flat_inj; rewrite pred_dec_true. auto. inv SPV; auto.
+  apply regs_inject_regs; auto. eauto.
+  auto.
 
 - (* tailcall *)
   exploit find_function_translated; eauto. intro FIND'.
-  exploit Mem.free_parallel_extends; eauto. intros [m'1 [FREE EXT]].
+  exploit Mem.free_parallel_inject; eauto.
+  unfold Mem.flat_inj; rewrite pred_dec_true; auto. inv SPV; auto. constructor.
+  intros [m'1 [FREE EXT]].
+  exploit Mem.unrecord_stack_block_inject_parallel. apply EXT. eauto.
+  {
+    red in CFG. simpl in CFG.
+    intros i j Gi LT.
+    eapply compat_frameinj_rec_above in Gi. 2: apply CFG. omega. omega.
+  }
+  {
+    apply CFG.
+  }
+  intros (m2' & USB' & UINJ).
   TransfInstr.
-  left. exists (Callstate s' (transf_fundef fd) (rs'##args) m'1); split.
-  eapply exec_Itailcall; eauto. apply sig_preserved.
-  rewrite stacksize_preserved; auto.
-  constructor. auto.  apply regs_lessdef_regs; auto. auto.
+  left. exists (Callstate s' (transf_fundef fd) (rs'##args) m2' (fn_stack_requirements id)); split.
+  eapply exec_Itailcall; eauto.
+  eapply ros_is_function_transf; eauto.
+  eapply meminj_preserves_globals_flat; eauto.
+  apply sig_preserved.
+  eauto. rewrite stacksize_preserved; auto. rewrite ! Z.add_0_r in FREE. eauto.
+  econstructor.
+  erewrite Mem.unrecord_stack_block_nextblock by eauto.
+  erewrite Mem.nextblock_free by eauto. eauto.
+  eauto.  apply regs_inject_regs; auto.
+  erewrite Mem.unrecord_stack_block_nextblock by eauto.
+  erewrite Mem.nextblock_free by eauto. eauto.
+  erewrite Mem.unrecord_stack_block_nextblock by eauto.
+  erewrite Mem.nextblock_free by eauto. eauto.
+  {
+    destruct CFG as (G0 & CFG).
+
+    Lemma compat_frameinj_rec_pop_parallel:
+      forall g l ns nt
+        (CFR: compat_frameinj_rec l g (S ns) (S nt)),
+        compat_frameinj_rec l (fun n : nat => option_map Init.Nat.pred (g (S n))) ns nt.
+    Proof.
+      induction l; simpl; intros; eauto.
+      - unfold option_map in Gi; repeat destr_in Gi.
+        eapply CFR in Heqo. omega. omega.
+      - destr; destruct CFR as (Gn & CFR).
+        + split.
+          * unfold option_map. rewrite Gn. reflexivity.
+          * eapply IHl; eauto.
+        + split.
+          * unfold option_map. rewrite Gn. reflexivity.
+          * eapply IHl; eauto.
+    Qed.
+    eapply compat_frameinj_rec_pop_parallel; eauto.
+
+  }
 
 - (* builtin *)
   TransfInstr.
-  exploit (eval_builtin_args_lessdef (ge := ge) (e1 := fun r => rs#r) (fun r => rs'#r)); eauto.
+  exploit (@eval_builtin_args_inject _ _ _ _ ge tge (fun r => rs#r) (fun r => rs'#r) (Vptr sp0 Ptrofs.zero)); eauto.
+  {
+    econstructor. unfold Mem.flat_inj. rewrite pred_dec_true; eauto. inv SPV; auto. reflexivity.
+  }
+  {
+    simpl. intros; rewrite symbols_preserved; auto.
+  }
+  {
+    simpl; intros.
+    generalize (meminj_preserves_globals_flat ge m). intro MPG. trim MPG; eauto.
+    destruct MPG; eauto.
+  }
   intros (vargs' & P & Q).
-  exploit external_call_mem_extends; eauto.
-  intros [v' [m'1 [A [B [C D]]]]].
+  exploit external_call_mem_inject; eauto.
+  eapply meminj_preserves_globals_flat; eauto.
+  intros [f' [v' [m'1 [A [B [C [D [E [F G]]]]]]]]].
   left. exists (State s' (transf_function f) (Vptr sp0 Ptrofs.zero) pc' (regmap_setres res v' rs') m'1); split.
   eapply exec_Ibuiltin; eauto.
-  eapply eval_builtin_args_preserved with (ge1 := ge); eauto. exact symbols_preserved.
+  edestruct eval_builtin_args_inject with (e1:= fun r => rs # r) (e2:= fun r => rs' # r) (sp1:=Vptr sp0 Ptrofs.zero) as
+      (args' & EVALargs' & INJargs); eauto.
+  {
+    econstructor. unfold Mem.flat_inj.  rewrite pred_dec_true; eauto. inv SPV; auto. reflexivity.
+  }
+  {
+    simpl; intros.
+    generalize (meminj_preserves_globals_flat ge m). intro MPG. trim MPG; eauto.
+    destruct MPG; eauto.
+  }
   eapply external_call_symbols_preserved; eauto. apply senv_preserved.
-  econstructor; eauto. apply set_res_lessdef; auto.
+  econstructor; eauto.
+  
+  apply set_res_inject; auto.
 
 - (* cond *)
   TransfInstr.
   left. exists (State s' (transf_function f) (Vptr sp0 Ptrofs.zero) (if b then ifso else ifnot) rs' m'); split.
   eapply exec_Icond; eauto.
-  apply eval_condition_lessdef with (rs##args) m; auto. apply regs_lessdef_regs; auto.
+  apply eval_condition_inject with (rs##args) m; auto. apply regs_inject_regs; auto.
   constructor; auto.
 
 - (* jumptable *)
@@ -517,7 +846,7 @@ Proof.
   constructor; auto.
 
 - (* return *)
-  exploit Mem.free_parallel_extends; eauto. intros [m'1 [FREE EXT]].
+  exploit Mem.free_parallel_inject; eauto. intros [m'1 [FREE EXT]].
   TransfInstr.
   left. exists (Returnstate s' (regmap_optget or Vundef rs') m'1); split.
   apply exec_Ireturn; auto. rewrite stacksize_preserved; auto.
@@ -530,17 +859,17 @@ Proof.
   right. split. simpl. omega. split. auto.
   constructor. auto.
   simpl. constructor.
-  eapply Mem.free_left_extends; eauto.
+  eapply Mem.free_left_inject; eauto.
 
 - (* eliminated return Some *)
   assert (or = Some r) by congruence. subst or.
   right. split. simpl. omega. split. auto.
   constructor. auto.
   simpl. auto.
-  eapply Mem.free_left_extends; eauto.
+  eapply Mem.free_left_inject; eauto.
 
 - (* internal call *)
-  exploit Mem.alloc_extends; eauto.
+  exploit Mem.alloc_inject; eauto.
     instantiate (1 := 0). omega.
     instantiate (1 := fn_stacksize f). omega.
   intros [m'1 [ALLOC EXT]].
@@ -552,10 +881,10 @@ Proof.
   left. econstructor; split.
   simpl. eapply exec_function_internal; eauto. rewrite EQ1; eauto.
   rewrite EQ2. rewrite EQ3. constructor; auto.
-  apply regs_lessdef_init_regs. auto.
+  apply regs_inject_init_regs. auto.
 
 - (* external call *)
-  exploit external_call_mem_extends; eauto.
+  exploit external_call_mem_inject; eauto.
   intros [res' [m2' [A [B [C D]]]]].
   left. exists (Returnstate s' res' m2'); split.
   simpl. econstructor; eauto.
@@ -567,7 +896,7 @@ Proof.
 + (* synchronous return in both programs *)
   left. econstructor; split.
   apply exec_return.
-  constructor; auto. apply set_reg_lessdef; auto.
+  constructor; auto. apply set_reg_inject; auto.
 + (* return instr in source program, eliminated because of tailcall *)
   right. split. unfold measure. simpl length.
   change (S (length s) * (niter + 2))%nat
@@ -590,7 +919,7 @@ Proof.
   rewrite symbols_preserved. eauto.
   symmetry; eapply match_program_main; eauto. 
   rewrite <- H3. apply sig_preserved.
-  constructor. constructor. constructor. apply Mem.extends_refl.
+  constructor. constructor. constructor. apply Mem.inject_refl.
 Qed.
 
 Lemma transf_final_states:
